SystemF/CBV/Safety.lean
@@ -1,0 +1,100 @@
+import SystemF.Lc.Tm
+import SystemF.Lc.TyTm
+import SystemF.Typing
+import SystemF.CBV.Semantics
+
+namespace SystemF.CBV
+
+open Notation
+
+theorem preservation {Γ : Context} {t t' : Tm} {T : Ty}
+    (hTyping : Γ ⊢ t ∶ T) (hStep : t ⟶ t') :
+    Γ ⊢ t' ∶ T := by
+  induction hStep generalizing T with
+  | app₁ t₁ t₁' t₂ _ _ _ =>
+    cases hTyping
+    constructor <;> aesop
+  | app₂ v t₂ t₂' _ _ _ =>
+    cases hTyping
+    constructor <;> aesop
+  | tApp t t' T _ _ _ =>
+    cases hTyping
+    constructor <;> aesop
+  | appLam t T v _ _ =>
+    cases hTyping with
+    | app Γ t₁ t₂ T₁ T₂ hT₁ hT₂ =>
+      cases hT₁ with
+      | lam L Γ T₁ T₂ t _ hBody =>
+        obtain ⟨x, hx⟩ := exists_fresh_name (L ∪ t.fv)
+        have hx₁ : x ∉ L := by aesop
+        have hx₂ : x ∉ t.fv := by aesop
+        rw [←substTm_openTm_var hx₂]
+        have := hBody x hx₁
+        have := typing_subst_tm (Γ₁ := []) (Γ₂ := Γ) this (by aesop)
+        simp only [List.nil_append] at this
+        exact this
+  | tAppTLam t T _ _ =>
+    cases hTyping with
+    | tApp Γ t T₁ T₂ hT₁ _ =>
+      cases hT₁ with
+      | tLam L Γ t T hBody =>
+        obtain ⟨X, hX⟩ := exists_fresh_name (L ∪ T₁.fv ∪ t.fvTy ∪ Γ.fv)
+        have hX₁ : X ∉ L := by aesop
+        have hX₂ : X ∉ T₁.fv := by aesop
+        have hX₃ : X ∉ t.fvTy := by aesop
+        have hX₄ : X ∉ Γ.fv := by aesop
+        rw [←substTy_openTy_var hX₂]
+        rw [←substTmTy_openTmTy_var hX₃]
+        have := hBody X hX₁
+        have := typing_subst_ty (Γ₁ := []) this (by assumption)
+        rw [substCtx_fresh hX₄] at this
+        exact this
+
+theorem progress {t : Tm} {T : Ty} (hTyping : ∅ ⊢ t ∶ T) :
+    Value t ∨ ∃ t', t ⟶ t' := by
+  generalize h : (∅ : Context) = Γ at hTyping
+  induction hTyping with (subst h)
+  | var Γ x T _ _ _ => contradiction
+  | lam L Γ T₁ T₂ t _ _ _ => left; constructor
+  | app Γ t₁ t₂ T₁ T₂ hTy₁ hTy₂ ih₁ ih₂ =>
+    simp_all only [List.empty_eq, forall_const]
+    cases ih₁ with
+    | inl hV₁ =>
+      cases ih₂ with
+      | inl hV₂ =>
+        obtain ⟨f, rfl⟩ := canonical_forms_arr hTy₁ hV₁
+        right
+        use f⟪t₂⟫
+        constructor
+        · exact typing_regularity_tm hTy₁
+        · assumption
+      | inr h =>
+        obtain ⟨t₂', hStep⟩ := h
+        right
+        use t₁ ◦ t₂'
+        constructor <;> assumption
+    | inr h =>
+      right
+      obtain ⟨t₁', hStep⟩ := h
+      use t₁' ◦ t₂
+      constructor
+      · exact typing_regularity_tm hTy₂
+      · assumption
+  | tLam L Γ t T _ _ => left; constructor
+  | tApp Γ t T₁ T₂ hTy _ ih =>
+    simp_all only [List.empty_eq, forall_const]
+    cases ih with
+    | inl hV =>
+      obtain ⟨f, rfl⟩ := canonical_forms_all hTy hV
+      right
+      use f⟪T₂⟫
+      constructor
+      · exact typing_regularity_tm hTy
+      · assumption
+    | inr h =>
+      obtain ⟨t', hStep⟩ := h
+      right
+      use t'⦃T₂⦄
+      constructor <;> assumption
+
+end SystemF.CBV
