SystemF/Lc.lean
@@ -1,0 +1,3 @@
+import SystemF.Lc.Ty
+import SystemF.Lc.Tm
+import SystemF.Lc.TyTm
