SystemF/Typing.lean
@@ -1,7 +1,10 @@
 import SystemF.Context
 import SystemF.Lc.Tm
+import SystemF.Lc.TyTm
 
 namespace SystemF
+
+open Notation
 
 /-- Typing relation -/
 @[aesop unsafe cases 20%]
@@ -142,5 +145,234 @@ lemma typing_regularity_wf {Γ t T} (h : Γ ⊢ t ∶ T) : WfContext Γ := by
     specialize ih X hX
     exact wf_remove_mid (Γ₁ := []) (Γ₂ := Γ) ih
   | tApp Γ t T₁ T₂ _ _ _ => assumption
+
+
+/-- Inserting a new variable into a well-formed context preserves well-formedness,
+  as long as the new variable is not free in the existing context.
+-/
+theorem typing_weakening {Γ₁ Γ₂ : Context} {t : Tm} {T : Ty} {x : Name} {b : Binding}
+    (hTyping : (Γ₁ ++ Γ₂) ⊢ t ∶ T)
+    (hWf : WfContext (Γ₁ ++ (x, b) :: Γ₂)) :
+    (Γ₁ ++ (x, b) :: Γ₂) ⊢ t ∶ T := by
+  generalize h : Γ₁ ++ Γ₂ = Γ at hTyping
+  induction hTyping generalizing Γ₁ with
+  | var Γ x T _ _ _ =>
+    subst h
+    constructor <;> aesop
+  | lam L Γ T₁ T₂ t _ _ ih =>
+    subst h
+    let ctx := (Γ₁ ++ (x, b) :: Γ₂)
+    apply HasType.lam (L ∪ ctx.dom)
+    · assumption
+    · intro y hy
+      have hy₁ : y ∉ L := by aesop
+      have hy₂ : y ∉ ctx.dom := by aesop
+      have hWf_new : WfContext ((y, .tm T₁) :: Γ₁ ++ (x, b) :: Γ₂) := by
+        constructor <;> assumption
+      exact ih y hy₁ hWf_new rfl
+  | app Γ t₁ t₂ T₁ T₂ _ _ ih₁ ih₂ =>
+    constructor
+    · apply ih₁ hWf h
+    · apply ih₂ hWf h
+  | tLam L Γ t T _ ih =>
+    subst h
+    let ctx := (Γ₁ ++ (x, b) :: Γ₂)
+    apply HasType.tLam (L ∪ ctx.dom)
+    intro Y hY
+    have hY₁ : Y ∉ L := by aesop
+    have hY₂ : Y ∉ ctx.dom := by aesop
+    have hWf_new : WfContext ((Y, .ty) :: Γ₁ ++ (x, b) :: Γ₂) := by
+      constructor <;> assumption
+    exact ih Y hY₁ hWf_new rfl
+  | tApp Γ t T₁ T₂ _ _ ih =>
+    constructor
+    · apply ih hWf h
+    · assumption
+
+
+/-- For `x : T` in `Γ`, substituting free variable `X` with `U` in `Γ`
+  yields `(x, T[X ↦ U])` in `Γ[X ↦ U]`.
+-/
+theorem substCtx_lookup {Γ : Context} {x : Name} {T U : Ty} {X : Name}
+    (h : (x, .tm T) ∈ Γ) :
+    (x, .tm T[X ↦ U]) ∈ Γ[X ↦ U] := by
+  induction Γ with
+  | nil => simp only [substCtx_nil, List.not_mem_nil]; contradiction
+  | cons head tail ih =>
+    simp only [List.mem_cons] at h
+    cases h with
+    | inl h =>
+      subst h
+      simp only [substCtx_cons_tm, List.mem_cons, true_or]
+    | inr h =>
+      simp_all only [forall_const]
+      rcases head with ⟨y, b⟩
+      cases b with
+      | ty => simp_all only [substCtx_cons_ty, List.mem_cons, Prod.mk.injEq, reduceCtorEq,
+        and_false, or_true]
+      | tm T => simp_all only [substCtx_cons_tm, List.mem_cons, Prod.mk.injEq, Binding.tm.injEq,
+        or_true]
+
+@[simp]
+lemma substCtx_dom {Γ : Context} {X : Name} {U : Ty} :
+    (Γ[X ↦ U]).dom = Γ.dom := by
+  induction Γ with
+  | nil => simp
+  | cons head tail ih =>
+    rcases head with ⟨y, b⟩
+    cases b with
+    | ty => simp_all only [substCtx_cons_ty, dom_cons, Finset.singleton_union]
+    | tm T => simp_all only [substCtx_cons_tm, dom_cons, Finset.singleton_union]
+
+lemma substCtx_wf {Γ : Context} {X : Name} {U : Ty}
+    (hWf : WfContext Γ) (hU : LcTy U) : WfContext (Γ[X ↦ U]) := by
+  induction hWf with
+  | nil => simp; constructor
+  | consTy Γ X _ _ ih =>
+    simp only [substCtx_cons_ty]
+    constructor
+    · assumption
+    · simp only [substCtx_dom]
+      assumption
+  | consTm Γ x T _ _ hLc ih =>
+    simp only [substCtx_cons_tm]
+    constructor
+    · assumption
+    · simp only [substCtx_dom]
+      assumption
+    · exact substTy_lcTy hLc hU
+
+/-- Substitution lemma for types -/
+theorem typing_subst_ty {Γ₁ Γ₂ : Context} {t : Tm} {T U : Ty} {X : Name}
+    (hTyping : (Γ₁ ++ (X, .ty) :: Γ₂) ⊢ t ∶ T)
+    (hLcTy : LcTy U) :
+    (Γ₁[X ↦ U] ++ Γ₂[X ↦ U]) ⊢ (t[X ↦ U]) ∶ (T[X ↦ U]) := by
+  generalize h : Γ₁ ++ (X, .ty) :: Γ₂ = Γ at hTyping
+  induction hTyping generalizing Γ₁ with
+  | var Γ x T hWf h₁ h₂ =>
+    subst h
+    constructor
+    · have := wf_remove_mid hWf
+      have := substCtx_wf this hLcTy (X := X)
+      simp only at this
+      rw [substCtx_append] at this
+      exact this
+    · simp only [List.mem_append, List.mem_cons, Prod.mk.injEq, reduceCtorEq, and_false,
+      false_or] at h₁
+      simp only [List.mem_append]
+      cases h₁ with
+      | inl h =>
+        left
+        apply substCtx_tm_mem
+        assumption
+      | inr h =>
+        right
+        apply substCtx_tm_mem
+        assumption
+    · exact substTy_lcTy h₂ hLcTy
+  | lam L Γ T₁ T₂ t h₁ h₂ ih =>
+    subst h
+    apply HasType.lam (L ∪ {X} ∪ U.fv)
+    · exact substTy_lcTy h₁ hLcTy
+    · intro y hy
+      have hy₁ : y ∉ L := by aesop
+      -- ((y, .tm (substTy X U T₁)) :: (Γ₁[X ↦ U] ++ Γ₂[X ↦ U])) ⊢
+      --  substTmTy X U t⟪$vy⟫ ∶ substTy X U T₂
+      change ((y, .tm T₁[X ↦ U]) :: (Γ₁[X ↦ U] ++ Γ₂[X ↦ U])) ⊢ (t[X ↦ U])⟪$vy⟫ ∶ (T₂[X ↦ U])
+      have := ih (Γ₁ := (y, Binding.tm T₁) :: Γ₁) y hy₁ rfl
+      rw [openTm_substTmTy_comm_fresh]
+      · exact this
+      simp [Tm.fvTy]
+  | app Γ t₁ t₂ T₁ T₂ _ _ ih₁ ih₂ =>
+    simp only [substTmTy_app]
+    constructor <;> aesop
+  | tLam L Γ t T _ ih =>
+    subst h
+    apply HasType.tLam (L ∪ {X} ∪ U.fv)
+    intro Y hY
+    -- ((Y, .ty) :: (Γ₁[X ↦ U] ++ Γ₂[X ↦ U])) ⊢ substTmTy X U t⟪$TY⟫ ∶ substTy X U T⟪$TY⟫
+    change ((Y, .ty) :: (Γ₁[X ↦ U] ++ Γ₂[X ↦ U])) ⊢ (t[X ↦ U])⟪$TY⟫ ∶ (T[X ↦ U])⟪$TY⟫
+    have hY₁ : Y ∉ L := by aesop
+    have hY₂ : X ≠ Y := by aesop
+    rw [openTy_substTy_comm hY₂ hLcTy]
+    rw [openTmTy_substTmTy_comm hY₂ hLcTy]
+    have := ih (Γ₁ := (Y, .ty) :: Γ₁) Y hY₁ rfl
+    exact this
+  | tApp Γ t T₁ T₂ _ _ ih =>
+    rw [substTy_dist_openTy hLcTy]
+    constructor
+    · aesop
+    · apply substTy_lcTy <;> assumption
+
+/-- Substitution lemma for terms -/
+theorem typing_subst_tm {Γ₁ Γ₂ : Context} {t u : Tm} {T U : Ty} {x : Name}
+    (hTyping : (Γ₁ ++ (x, .tm U) :: Γ₂) ⊢ t ∶ T)
+    (hSubstTyping : (Γ₁ ++ Γ₂) ⊢ u ∶ U) :
+    (Γ₁ ++ Γ₂) ⊢ (t[x ↦ u]) ∶ T := by
+  generalize h : Γ₁ ++ (x, .tm U) :: Γ₂ = Γ at hTyping
+  induction hTyping generalizing Γ₁ with
+  | var Γ x' T _ _ _ =>
+    simp only [substTm_fvar, beq_iff_eq]
+    split
+    · simp_all only
+      rename_i hWf mem _ _
+      subst h
+      have : Binding.tm T = Binding.tm U := wf_lookup_mid hWf mem
+      have : T = U := by injection this
+      rw [this]
+      assumption
+    · subst h
+      constructor
+      · exact typing_regularity_wf hSubstTyping
+      · aesop
+      · assumption
+  | lam L Γ T₁ T₂ t _ _ ih =>
+    simp only [substTm_lam]
+    apply HasType.lam (L ∪ {x} ∪ (Context.dom Γ))
+    · assumption
+    · intro y hy
+      have hLCu : LcTm u := typing_regularity_tm hSubstTyping
+      have hy₁ : y ∉ L := by aesop
+      have hy₂ : y ≠ x := by aesop
+      have hy₃ : y ∉ Context.dom (Γ₁ ++ Γ₂) := by aesop
+      rw [openTm_substTm_comm_of_neq hy₂ hLCu]
+      have : ((y, .tm T₁) :: Γ₁ ++ Γ₂) ⊢ u ∶ U := by
+        have := typing_weakening (Γ₁ := []) (Γ₂ := Γ₁ ++ Γ₂) (x := y) (b := .tm T₁) hSubstTyping
+        simp only [List.nil_append] at this
+        apply this
+        constructor
+        · exact typing_regularity_wf hSubstTyping
+        · exact hy₃
+        · assumption
+      -- Γ₁ ++ (x, .tm U) :: Γ₂ = (y, .tm T₁) :: (Γ₁ ++ (x, .tm U) :: Γ₂)
+      exact @ih y hy₁ ((y, .tm T₁) :: Γ₁) this (by aesop)
+  | app Γ t₁ t₂ T₁ T₂ _ _ ih₁ ih₂ =>
+    subst h
+    simp only [substTm_app]
+    constructor
+    · apply ih₁
+      · assumption
+      · rfl
+    · apply ih₂
+      · assumption
+      · rfl
+  | tLam L Γ t T _ ih =>
+    simp only [substTm_tLam]
+    apply HasType.tLam (L ∪ Context.dom Γ)
+    intro Y hY
+    have hLCu : LcTm u := typing_regularity_tm hSubstTyping
+    have hY₁ : Y ∉ L := by aesop
+    have hY₂ : Y ∉ Context.dom (Γ₁ ++ Γ₂) := by aesop
+    rw [←openTmTy_substTm_comm hLCu]
+    rw [←List.cons_append]
+    apply ih
+    · assumption
+    · have : WfContext (Γ₁ ++ Γ₂) := typing_regularity_wf hSubstTyping
+      exact typing_weakening (Γ₁ := []) hSubstTyping (by constructor <;> assumption)
+    · aesop
+  | tApp Γ t T₁ T₂ _ _ ih =>
+    constructor
+    apply ih <;> assumption
+    assumption
 
 end SystemF
